Update to v4.32.0-rc1

Smt/Reconstruct/Int/Lemmas.lean
@@ -11,7 +11,7 @@ private theorem Int.mul_eq_zero_left {x y : Int} (hx : x ≠ 0) (hxy : x * y = 0
   rewrite [Int.mul_eq_zero] at hxy
   exact hxy.resolve_left hx
 
-private def uncurry {p₁ p₂ p₃ : Prop} : (p₁ → p₂ → p₃) → (p₁ ∧ p₂) → p₃ := by
+private theorem uncurry {p₁ p₂ p₃ : Prop} : (p₁ → p₂ → p₃) → (p₁ ∧ p₂) → p₃ := by
   intros h₁ h₂
   have ⟨ht₁, ht₂⟩ := h₂
   exact h₁ ht₁ ht₂
